doc/coq/Linking.v
@@ -223,7 +223,8 @@ Qed.
   update_lt := link_update_lt
 }.
 
-Fixpoint lift_ctx_bf `{OrderT BT} (C : @dy_ctx BT) :=
+Fixpoint lift_ctx_bf `{EB : Eq BT} `{EA : Eq AT} (C : @dy_ctx BT) 
+  : @dy_ctx (@link BT EB AT EA) :=
   match C with
   | ([||]) => ([||])
   | dy_c_lam x t C' => dy_c_lam x (BF t) (lift_ctx_bf C')
@@ -231,7 +232,8 @@ Fixpoint lift_ctx_bf `{OrderT BT} (C : @dy_ctx BT) :=
   | dy_c_letm M C' C'' => dy_c_letm M (lift_ctx_bf C') (lift_ctx_bf C'')
   end.
 
-Fixpoint lift_ctx_af `{OrderT AT} (C : @dy_ctx AT) :=
+Fixpoint lift_ctx_af `{EB : Eq BT} `{EA : Eq AT} (C : @dy_ctx AT)
+  : @dy_ctx (@link BT EB AT EA) :=
   match C with
   | ([||]) => ([||])
   | dy_c_lam x t C' => dy_c_lam x (AF t) (lift_ctx_af C')
@@ -239,19 +241,386 @@ Fixpoint lift_ctx_af `{OrderT AT} (C : @dy_ctx AT) :=
   | dy_c_letm M C' C'' => dy_c_letm M (lift_ctx_af C') (lift_ctx_af C'')
   end.
 
-Fixpoint inject_ctx {T} (Cout : @dy_ctx T) (Cin : @dy_ctx T) :=
+Fixpoint map_inject {T} (Cout : @dy_ctx T) (Cin : @dy_ctx T) :=
   match Cin with
-  | ([||]) => Cout
+  | [||] => [||]
   | dy_c_lam x t C' =>
-    inject_ctx (Cout [|dy_c_lam x t ([||])|]) C'
+    dy_c_lam x t (map_inject Cout C')
   | dy_c_lete x t C' =>
-    inject_ctx (Cout [|dy_c_lete x t ([||])|]) C'
-  | dy_c_letm M C' C'' => 
-    inject_ctx (Cout [|dy_c_letm M (inject_ctx Cout C') ([||])|]) C''
+    dy_c_lete x t (map_inject Cout C')
+  | dy_c_letm M C' C'' =>
+    dy_c_letm M (Cout[|map_inject Cout C'|]) (map_inject Cout C'')
   end.
 
+Definition inject_ctx {T} (Cout : @dy_ctx T) (Cin : @dy_ctx T) :=
+  Cout[|map_inject Cout Cin|].
+
+Fixpoint delete_prefix {T} `{Eq T} (Cout : @dy_ctx T) (Cin : @dy_ctx T) :=
+  match Cout, Cin with
+  | [||], Cin => Cin
+  | dy_c_lam x t Cout', dy_c_lam x' t' Cin'
+  | dy_c_lete x t Cout', dy_c_lete x' t' Cin' =>
+    if eq_eid x x' && eqb t t' then
+      delete_prefix Cout' Cin'
+    else Cin
+  | dy_c_letm M Cout' Cout'', dy_c_letm M' Cin' Cin'' =>
+    if eq_mid M M' && eq_ctx Cout' Cin' then
+      delete_prefix Cout'' Cin''
+    else Cin
+  | _, _ => Cin
+  end.
+
+Ltac intro_refl :=
+  assert (forall x, eq_eid x x = true) as eid_refl; [intros; apply eq_eid_eq; eauto|idtac];
+  assert (forall M, eq_mid M M = true) as mid_refl; [intros; apply eq_mid_eq; eauto|idtac];
+  assert (forall {T} `{Eq T} t, eqb t t = true) as t_refl; [intros; apply eqb_eq; eauto|idtac];
+  assert (forall {T} `{Eq T} C, eq_ctx C C = true) as ctx_refl; [intros; apply eq_ctx_eq; eauto|idtac].
+
+Lemma delete_prefix_eq :
+  forall {T} `{Eq T} (Cout Cin : dy_ctx),
+    delete_prefix Cout (Cout[|Cin|]) = Cin.
+Proof.
+  intro_refl. intros. rename H into ET. revert Cin.
+  induction Cout; simpl; eauto;    
+    try rewrite eid_refl; try rewrite mid_refl; try rewrite t_refl; try rewrite ctx_refl;
+    simpl; eauto.
+Qed.
+
+Lemma delete_prefix_dec :
+  forall {T} `{Eq T} (Cout Cin : @dy_ctx T),
+    dy_level (delete_prefix Cout Cin) <= dy_level Cin.
+Proof.
+  intros. revert Cout. 
+  induction Cin; intros; destruct Cout; simpl; eauto;
+  try destruct (eq_eid x0 x); try destruct (eqb tx0 tx);
+  try destruct (eq_mid M0 M); try destruct (eq_ctx Cout1 Cin1);
+  simpl; try nia.
+  etransitivity; try apply IHCin; eauto.
+  etransitivity; try apply IHCin; eauto.
+  etransitivity; try apply IHCin2; nia.
+Qed.
+
+Require Import Program.
+
+Program Fixpoint delete_map 
+  {T} `{Eq T} (Cout Cin : dy_ctx) {measure (dy_level Cin)} :=
+  match Cin with
+  | [||] => [||]
+  | dy_c_lam x t C' =>
+    dy_c_lam x t (delete_map Cout C')
+  | dy_c_lete x t C' =>
+    dy_c_lete x t (delete_map Cout C')
+  | dy_c_letm M C' C'' =>
+    dy_c_letm M (delete_map Cout (delete_prefix Cout C'))
+                (delete_map Cout C'')
+  end.
+
+Next Obligation.
+  simpl.
+  pose proof (delete_prefix_dec Cout C').
+  nia.
+Defined.
+Next Obligation.
+  simpl.
+  pose proof (delete_prefix_dec Cout C'').
+  nia.
+Defined.
+
+(* reduction lemmas *)
+Lemma delete_map_red_lam :
+  forall {T} `{Eq T} Cout x t C',
+    delete_map Cout (dy_c_lam x t C') =
+      dy_c_lam x t (delete_map Cout C').
+Proof.
+  intros. unfold delete_map. unfold delete_map_func.
+  rewrite fix_sub_eq; simpl; try reflexivity.
+  intros x' f g Heq.
+  specialize (functional_extensionality_dep f g Heq).
+  intros RR. rewrite RR. reflexivity.
+Qed.
+
+Lemma delete_map_red_lete :
+  forall {T} `{Eq T} Cout x t C',
+    delete_map Cout (dy_c_lete x t C') =
+      dy_c_lete x t (delete_map Cout C').
+Proof.
+  intros. unfold delete_map. unfold delete_map_func.
+  rewrite fix_sub_eq; simpl; try reflexivity.
+  intros x' f g Heq.
+  specialize (functional_extensionality_dep f g Heq).
+  intros RR. rewrite RR. reflexivity.
+Qed.
+
+Lemma delete_map_red_letm :
+  forall {T} `{Eq T} Cout M C' C'',
+    delete_map Cout (dy_c_letm M C' C'') =
+      dy_c_letm M (delete_map Cout (delete_prefix Cout C'))
+                  (delete_map Cout C'').
+Proof.
+  intros. unfold delete_map. unfold delete_map_func.
+  rewrite fix_sub_eq; simpl; try reflexivity.
+  intros x' f g Heq.
+  specialize (functional_extensionality_dep f g Heq).
+  intros RR. rewrite RR. reflexivity.
+Qed.
+
+Ltac simpl_delete :=
+  simpl;
+  try rewrite delete_map_red_lam;
+  try rewrite delete_map_red_lete;
+  try rewrite delete_map_red_letm.
+
+Lemma delete_map_eq :
+  forall {T} `{Eq T} (Cout Cin : dy_ctx),
+    delete_map Cout (map_inject Cout Cin) = Cin.
+Proof.
+  intros. rename H into ET. revert Cout.
+  induction Cin; intros; simpl_delete; 
+  try rewrite IHCin; eauto.
+  rewrite delete_prefix_eq. 
+  rewrite IHCin1. rewrite IHCin2. eauto.
+Qed.
+
+Definition delete_inject {T} `{Eq T} (Cout Cin : dy_ctx) :=
+  delete_map Cout (delete_prefix Cout Cin).
+
+Lemma delete_inject_eq :
+  forall {T} `{Eq T} (Cout Cin : dy_ctx),
+    delete_inject Cout (inject_ctx Cout Cin) = Cin.
+Proof.
+  intros. unfold delete_inject. unfold inject_ctx.
+  rewrite delete_prefix_eq.
+  rewrite delete_map_eq. eauto.
+Qed.
+  
 Notation "Cout '<|' Cin '|>'" := (inject_ctx Cout Cin)
                               (at level 100, Cin at next level, right associativity).
+
+Definition inject_ctx_mem {T} `{Eq T} (Cout : @dy_ctx T) (mem : T -> option (@expr_value T)) :=
+  fun t =>
+    match mem t with
+    | Some (Closure x t C) => Some (Closure x t (Cout <|C|>))
+    | None => None
+    end.
+
+Definition delete_ctx_mem {T} `{Eq T} (Cout : @dy_ctx T) (mem : T -> option (@expr_value T)) :=
+  fun t =>
+    match mem t with
+    | Some (Closure x t C) => Some (Closure x t (delete_inject Cout C))
+    | None => None
+    end.
+
+Lemma delete_ctx_mem_eq :
+  forall {T} `{Eq T} (Cout : @dy_ctx T) (mem : T -> option (@expr_value T)),
+         delete_ctx_mem Cout (inject_ctx_mem Cout mem) = mem.
+Proof.
+  intros. apply functional_extensionality.
+  intros. unfold inject_ctx_mem. unfold delete_ctx_mem.
+  destruct (mem x) eqn:ACCESS; try reflexivity.
+  destruct e. rewrite delete_inject_eq. reflexivity.
+Qed.
+
+Lemma map_inject_addr_x :
+  forall {T} `{Eq T} x (Cout : @dy_ctx T) (Cin : @dy_ctx T),
+    addr_x (map_inject Cout Cin) x = addr_x Cin x.
+Proof.
+  intros. revert Cout. 
+  induction Cin; intros; simpl; eauto;
+  destruct (addr_x Cin x) eqn:ADDR;
+  rewrite IHCin; eauto.
+Qed.
+
+Lemma map_inject_ctx_M :
+  forall {T} `{Eq T} M (Cout : @dy_ctx T) (Cin : @dy_ctx T),
+    ctx_M (map_inject Cout Cin) M =
+    match ctx_M Cin M with
+    | Some CM => Some (Cout <| CM |>)
+    | None => None
+    end.
+Proof.
+  intros. revert Cout.
+  induction Cin; intros; simpl; eauto.
+  rewrite IHCin2. destruct (ctx_M Cin2 M); eauto.
+  destruct (eq_mid M M0); eauto.
+Qed.
+
+Lemma plugin_ctx_addr_x :
+  forall {T} `{Eq T} x (Cout : @dy_ctx T) (Cin : @dy_ctx T),
+    match addr_x Cin x with
+    | Some t => addr_x (Cout[|Cin|]) x = Some t
+    | None => True
+    end.
+Proof.
+  intros. revert Cin.
+  induction Cout; intros; 
+  destruct (addr_x Cin x) eqn:ADDR; simpl; eauto;
+  try (specialize (IHCout Cin); rewrite ADDR in IHCout;
+      rewrite IHCout; eauto).
+  specialize (IHCout2 Cin); rewrite ADDR in IHCout2; rewrite IHCout2; eauto.
+Qed.
+
+Lemma plugin_ctx_ctx_M :
+  forall {T} `{Eq T} M (Cout : @dy_ctx T) (Cin : @dy_ctx T),
+    match ctx_M Cin M with
+    | Some CM => ctx_M (Cout[|Cin|]) M = Some CM
+    | None => True
+    end.
+Proof.
+  intros. revert Cin.
+  induction Cout; intros;
+  destruct (ctx_M Cin M) eqn:CTX; simpl; eauto;
+  try (specialize (IHCout Cin); rewrite CTX in IHCout;
+      rewrite IHCout; eauto).
+  specialize (IHCout2 Cin); rewrite CTX in IHCout2; rewrite IHCout2; eauto.
+Qed.
+
+Lemma inject_ctx_addr_x :
+  forall {T} `{Eq T} x (Cout : @dy_ctx T) (Cin : @dy_ctx T),
+    match addr_x Cin x with
+    | Some t => addr_x (Cout<|Cin|>) x = Some t
+    | None => True
+    end.
+Proof.
+  intros. destruct (addr_x Cin x) eqn:ADDR; eauto.
+  rewrite <- map_inject_addr_x with (Cout := Cout) in ADDR.
+  rewrite <- ADDR. 
+  pose proof plugin_ctx_addr_x.
+  specialize (H0 x Cout (map_inject Cout Cin)).
+  rewrite ADDR in H0. rewrite <- H0 in ADDR.
+  eauto.
+Qed.
+
+Lemma inject_ctx_ctx_M :
+  forall {T} `{Eq T} M (Cout : @dy_ctx T) (Cin : @dy_ctx T),
+    match ctx_M Cin M with
+    | Some CM => ctx_M (Cout<|Cin|>) M = Some (Cout <|CM|>)
+    | None => True
+    end.
+Proof.
+  intros. destruct (ctx_M Cin M) eqn:CTX; eauto.
+  pose proof (map_inject_ctx_M M Cout Cin).
+  rewrite CTX in H0.
+  pose proof (plugin_ctx_ctx_M M Cout (map_inject Cout Cin)).
+  rewrite H0 in H1. eauto.
+Qed.
+
+Definition delete_update {T} `{ET : Eq T} `{OT : @OrderT T ET} `{@time T ET OT} (Cout : @dy_ctx T) :=
+  fun C st x v =>
+    let delete_C := delete_inject Cout C in
+    let delete_st :=
+      match st with
+      | ST mem t => ST (delete_ctx_mem Cout mem) t
+      end in
+    let delete_v := 
+      match v with
+      | Closure x_v e_v C_v =>
+        Closure x_v e_v (delete_inject Cout C_v)
+      end in
+    update delete_C delete_st x delete_v.
+
+Lemma delete_update_lt {T} `{ET : Eq T} `{OT : @OrderT T ET} `{@time T ET OT} (Cout : @dy_ctx T) :
+  forall C mem t x v, let t' := delete_update Cout C (ST mem t) x v in
+                                leb t t' = true /\ eqb t t' = false.
+Proof.
+  intros. unfold delete_update in t'. apply update_lt.
+Qed.
+
+#[export] Instance delete_time {T} `{ET : Eq T} `{OT : @OrderT T ET} `{@time T ET OT} (Cout : @dy_ctx T) : @time T ET OT :=
+  {
+    update := delete_update Cout;
+    update_lt := delete_update_lt Cout
+  }.
+
+Lemma delete_update_eq {T} `{ET : Eq T} `{OT : @OrderT T ET} `{@time T ET OT} (Cout : @dy_ctx T) :
+  forall C mem t x v,
+    let inject_v :=
+      match v with
+      | Closure x_v e_v C_v => Closure x_v e_v (Cout<|C_v|>)
+      end in
+    delete_update Cout (Cout<|C|>) (ST (inject_ctx_mem Cout mem) t) x inject_v =
+    update C (ST mem t) x v.
+Proof.
+  intros. destruct v. destruct inject_v eqn:INJ. inversion INJ. subst.
+  unfold delete_update. rewrite delete_inject_eq. rewrite delete_ctx_mem_eq.
+  rewrite delete_inject_eq. reflexivity.
+Qed.
+
+Lemma plugin_map_assoc :
+  forall {T} `{Eq T} (Cout C C' : @dy_ctx T),
+    (map_inject Cout C) [|map_inject Cout C'|] = (map_inject Cout (C [|C'|])).
+Proof.
+  intros. revert Cout C'. induction C; intros; simpl; eauto; try rewrite IHC; try rewrite IHC2; eauto.
+Qed.
+
+Lemma plugin_inject_assoc :
+  forall {T} `{Eq T} (Cout C C' : @dy_ctx T),
+    (Cout <| C |>)[| map_inject Cout C' |] = (Cout <|C[|C'|]|>).
+Proof.
+  intros. unfold inject_ctx. rewrite <- c_plugin_assoc.
+  rewrite plugin_map_assoc. eauto.
+Qed.
+
+Lemma inject_update_m_eq :
+  forall {T} `{Eq T} t x e mem (Cout C : @dy_ctx T),
+  (t !-> Closure x e (Cout <| C |>); inject_ctx_mem Cout mem) =
+            inject_ctx_mem Cout (t !-> Closure x e C; mem).
+Proof.
+  intros. apply functional_extensionality.
+  intros. unfold update_m. unfold inject_ctx_mem.
+  destruct (eqb x0 t); eauto.
+Qed.
+
+Lemma delete_eval_eq {T} `{ET : Eq T} `{OT : @OrderT T ET} `{TT : @time T ET OT} (Cout : @dy_ctx T) :
+  forall C st e v st'
+         (EVAL : @EvalR T ET OT TT C st e v st'),
+    let inject_v :=
+      match v with
+      | EVal (Closure x_v e_v C_v) => EVal (Closure x_v e_v (Cout<|C_v|>))
+      | MVal C_v => MVal (Cout<|C_v|>)
+      end in
+    let inject_st :=
+      match st with
+      | ST mem t => ST (inject_ctx_mem Cout mem) t
+      end in
+    let inject_st' :=
+      match st' with
+      | ST mem' t' => ST (inject_ctx_mem Cout mem') t'
+      end in
+    @EvalR T ET OT (@delete_time T ET OT TT Cout)
+      (Cout<|C|>) inject_st e inject_v inject_st'.
+Proof.
+  intros. induction EVAL;
+  try destruct v; try destruct st; try destruct st'; try destruct st'';
+  try (destruct inject_v eqn:INJv; inversion INJv; subst);
+  try (destruct inject_st eqn:INJst; inversion INJst; subst);
+  try (destruct inject_st' eqn:INJst'; inversion INJst'; subst); eauto.
+  - inversion STATE; subst.
+    eapply Eval_var_e; eauto.
+    pose proof (inject_ctx_addr_x x Cout C) as RR.
+    rewrite <- ADDR in RR. symmetry. apply RR.
+    unfold inject_ctx_mem. rewrite <- ACCESS. eauto.
+  - destruct st_v. destruct arg.
+    eapply Eval_app. apply IHEVAL1. apply IHEVAL2.
+    pose proof (delete_update_eq Cout C mem t x (Closure x1 e3 C1)) as RR.
+    simpl in *. rewrite RR. clear RR.
+    rewrite inject_update_m_eq.
+    replace (dy_c_lam x t ([||])) with (map_inject Cout (dy_c_lam x t ([||]))) by reflexivity.
+    rewrite plugin_inject_assoc. eauto.
+  - pose proof (inject_ctx_ctx_M M Cout C) as RR. 
+    rewrite <- ACCESS in RR.
+    eapply Eval_var_m; eauto.
+  - eapply Eval_lete; eauto.
+    pose proof (delete_update_eq Cout C mem t x (Closure x0 e0 C0)) as RR.
+    simpl in *. rewrite RR. clear RR.
+    rewrite inject_update_m_eq.
+    replace (dy_c_lete x t ([||])) with (map_inject Cout (dy_c_lete x t ([||]))) by reflexivity.
+    rewrite plugin_inject_assoc. eauto.
+  - eapply Eval_letm; eauto.
+    assert ((Cout <| C |>) [|dy_c_letm M (Cout <| C' |>) ([||])|] =
+            (Cout <| (C [|dy_c_letm M C' ([||])|]) |>)) as RR. 
+    { rewrite <- plugin_inject_assoc. simpl. eauto. } 
+    rewrite RR. clear RR. simpl in *. exact IHEVAL2.
+Qed.
 
 Fixpoint lift_state_bf `{OrderT BT} (st : @state BT) :=
   match C with
